flake.nix
@@ -20,8 +20,7 @@
         devShell = mkShell rec {
           buildInputs = with coqPackages_8_19; [
             coq
-
-          # coq-lsp.packages.${system}.coq-lsp
+            coq-lsp
           ];
         };
       }
